Rename Stackless to Smart

Uppaal_Networks/AbsInt/State_Smart.thy
@@ -1,25 +1,25 @@
-theory State_Stackless
+theory State_Smart
   imports AbsInt ListLattice Toption Stack State_Option PowerBool Uppaal_Networks.UPPAAL_Asm_Map
 begin
 
 type_synonym 'a arstate = "'a list toption"
 
-datatype 'a stackless_base = Stackless "'a arstate" power_bool
-type_synonym 'a stackless = "'a stackless_base option"
+datatype 'a smart_base = Smart "'a arstate" power_bool
+type_synonym 'a smart = "'a smart_base option"
 
-instantiation stackless_base :: (absword) order_top
+instantiation smart_base :: (absword) order_top
 begin
-  definition[simp]: "\<top> \<equiv> Stackless \<top> \<top>"
+  definition[simp]: "\<top> \<equiv> Smart \<top> \<top>"
 
-  fun less_eq_stackless_base :: "'a stackless_base \<Rightarrow> 'a stackless_base \<Rightarrow> bool" where
-    "less_eq_stackless_base (Stackless aregs aflag) (Stackless bregs bflag) \<longleftrightarrow> aregs \<le> bregs \<and> aflag \<le> bflag"
+  fun less_eq_smart_base :: "'a smart_base \<Rightarrow> 'a smart_base \<Rightarrow> bool" where
+    "less_eq_smart_base (Smart aregs aflag) (Smart bregs bflag) \<longleftrightarrow> aregs \<le> bregs \<and> aflag \<le> bflag"
 
-  fun less_stackless_base :: "'a stackless_base \<Rightarrow> 'a stackless_base \<Rightarrow> bool" where
-    "less_stackless_base a b \<longleftrightarrow> a \<le> b \<and> \<not> b \<le> a"
+  fun less_smart_base :: "'a smart_base \<Rightarrow> 'a smart_base \<Rightarrow> bool" where
+    "less_smart_base a b \<longleftrightarrow> a \<le> b \<and> \<not> b \<le> a"
 instance
 proof (standard, goal_cases)
   case (2 x)
-  then show ?case using State_Stackless.less_eq_stackless_base.elims(3) by fastforce
+  then show ?case using State_Smart.less_eq_smart_base.elims(3) by fastforce
 next
   case (3 x y z) then show ?case by (cases x; cases y; cases z; auto)
 next
@@ -29,11 +29,11 @@ next
 qed simp
 end
 
-instantiation stackless_base :: (absword) semilattice_sup
+instantiation smart_base :: (absword) semilattice_sup
 begin
-  fun sup_stackless_base :: "'a stackless_base \<Rightarrow> 'a stackless_base \<Rightarrow> 'a stackless_base" where
-    "sup_stackless_base (Stackless aregs aflag) (Stackless bregs bflag) =
-      Stackless (aregs \<squnion> bregs) (aflag \<squnion> bflag)"
+  fun sup_smart_base :: "'a smart_base \<Rightarrow> 'a smart_base \<Rightarrow> 'a smart_base" where
+    "sup_smart_base (Smart aregs aflag) (Smart bregs bflag) =
+      Smart (aregs \<squnion> bregs) (aflag \<squnion> bflag)"
 instance
 proof (standard, goal_cases)
   case (1 x y) show ?case by (cases x; cases y; simp)
@@ -85,50 +85,50 @@ qed
 
 lemma mono_gamma_power_bool: "a \<le> b \<Longrightarrow> \<gamma>_power_bool a \<le> \<gamma>_power_bool b" by (cases a; cases b; simp)
 
-fun \<gamma>_stackless :: "'a stackless \<Rightarrow> collect_state set" where
-  "\<gamma>_stackless None = \<bottom>" |
-  "\<gamma>_stackless (Some (Stackless aregs aflag)) = {(stack, rstate, flag, nl). rstate \<in> \<gamma>_regs aregs \<and> flag \<in> \<gamma>_power_bool aflag}"
+fun \<gamma>_smart :: "'a smart \<Rightarrow> collect_state set" where
+  "\<gamma>_smart None = \<bottom>" |
+  "\<gamma>_smart (Some (Smart aregs aflag)) = {(stack, rstate, flag, nl). rstate \<in> \<gamma>_regs aregs \<and> flag \<in> \<gamma>_power_bool aflag}"
 
-fun step_stackless_base :: "instr \<Rightarrow> addr \<Rightarrow> 'a stackless_base \<Rightarrow> 'a stackless state_map" where
-  "step_stackless_base (JMPZ target) pc (Stackless regs BTrue)  = single (Suc pc) (Some (Stackless regs BTrue))" |
-  "step_stackless_base (JMPZ target) pc (Stackless regs BFalse) = single target (Some (Stackless regs BFalse))" |
-  "step_stackless_base (JMPZ target) pc (Stackless regs BBoth)  = deep_merge {(target, Some (Stackless regs BBoth)), (Suc pc, Some (Stackless regs BBoth))}" |
-  "step_stackless_base ADD           pc (Stackless regs flag)   = single (Suc pc) (Some (Stackless regs flag))" |
-  "step_stackless_base NOT           pc (Stackless regs flag)   = single (Suc pc) (Some (Stackless regs (not flag)))" |
-  "step_stackless_base AND           pc (Stackless regs flag)   = single (Suc pc) (Some (Stackless regs BBoth))" |
-  "step_stackless_base _ _ _ = \<top>"
+fun step_smart_base :: "instr \<Rightarrow> addr \<Rightarrow> 'a smart_base \<Rightarrow> 'a smart state_map" where
+  "step_smart_base (JMPZ target) pc (Smart regs BTrue)  = single (Suc pc) (Some (Smart regs BTrue))" |
+  "step_smart_base (JMPZ target) pc (Smart regs BFalse) = single target (Some (Smart regs BFalse))" |
+  "step_smart_base (JMPZ target) pc (Smart regs BBoth)  = deep_merge {(target, Some (Smart regs BBoth)), (Suc pc, Some (Smart regs BBoth))}" |
+  "step_smart_base ADD           pc (Smart regs flag)   = single (Suc pc) (Some (Smart regs flag))" |
+  "step_smart_base NOT           pc (Smart regs flag)   = single (Suc pc) (Some (Smart regs (not flag)))" |
+  "step_smart_base AND           pc (Smart regs flag)   = single (Suc pc) (Some (Smart regs BBoth))" |
+  "step_smart_base _ _ _ = \<top>"
 
-fun step_stackless :: "('a::absword) stackless astep" where
-  "step_stackless _ _ None = \<bottom>" |
-  "step_stackless op pc (Some a) = step_stackless_base op pc a"
+fun step_smart :: "('a::absword) smart astep" where
+  "step_smart _ _ None = \<bottom>" |
+  "step_smart op pc (Some a) = step_smart_base op pc a"
 
-lemma gamma_stackless_mono:
+lemma gamma_smart_mono:
   assumes "a \<le> b"
-  shows "\<gamma>_stackless a \<subseteq> \<gamma>_stackless b"
+  shows "\<gamma>_smart a \<subseteq> \<gamma>_smart b"
 proof (intro Set.subsetI)
-  fix x assume ass: "x \<in> \<gamma>_stackless a"
-  from ass obtain aregs aflag where asplit: "a = Some (Stackless aregs aflag)" by (metis \<gamma>_stackless.elims empty_iff)
-  from this assms obtain bregs bflag where bsplit: "b = Some (Stackless bregs bflag)" by (metis \<gamma>_stackless.cases less_eq_option.simps(2))
+  fix x assume ass: "x \<in> \<gamma>_smart a"
+  from ass obtain aregs aflag where asplit: "a = Some (Smart aregs aflag)" by (metis \<gamma>_smart.elims empty_iff)
+  from this assms obtain bregs bflag where bsplit: "b = Some (Smart bregs bflag)" by (metis \<gamma>_smart.cases less_eq_option.simps(2))
   from ass obtain stack rstate flag nl where xsplit: "x = (stack, rstate, flag, nl)" using prod_cases4 by blast 
   from assms asplit bsplit have fine_le: "aregs \<le> bregs" "aflag \<le> bflag" by auto
   from asplit xsplit ass have "rstate \<in> \<gamma>_regs aregs \<and> flag \<in> \<gamma>_power_bool aflag" by simp
   from this fine_le have "rstate \<in> \<gamma>_regs bregs" "flag \<in> \<gamma>_power_bool bflag" using mono_gamma_power_bool mono_gamma_regs by (blast, blast)
-  from this bsplit xsplit show "x \<in> \<gamma>_stackless b" by simp
+  from this bsplit xsplit show "x \<in> \<gamma>_smart b" by simp
 qed
 
-lemma gamma_stackless_top: "\<gamma>_stackless \<top> = \<top>"
+lemma gamma_smart_top: "\<gamma>_smart \<top> = \<top>"
 proof -
   have "rstate \<in> \<gamma>_regs \<top>" "flag \<in> \<gamma>_power_bool \<top>" for rstate flag by auto
   then show ?thesis by auto
 qed
 
-lemma step_stackless_nonbot_correct:
-  assumes "ost \<in> lookup (collect_step op ipc (\<gamma>_stackless (Some (Stackless iaregs iaflag)))) opc"
-  shows "ost \<in> \<gamma>_stackless (lookup (step_stackless op ipc (Some (Stackless iaregs iaflag))) opc)"
+lemma step_smart_nonbot_correct:
+  assumes "ost \<in> lookup (collect_step op ipc (\<gamma>_smart (Some (Smart iaregs iaflag)))) opc"
+  shows "ost \<in> \<gamma>_smart (lookup (step_smart op ipc (Some (Smart iaregs iaflag))) opc)"
 proof -
   obtain ocstack ocregs ocflag ocrs where ost_split: "ost = (ocstack, ocregs, ocflag, ocrs)" by (rule prod_cases4)
 
-  let ?ists = "\<gamma>_stackless (Some (Stackless iaregs iaflag))"
+  let ?ists = "\<gamma>_smart (Some (Smart iaregs iaflag))"
   from assms have "\<exists>ist\<in>?ists. step op (ipc, ist) = Some (opc, ost)" by simp
   from this obtain ist where ist_step: "ist \<in> ?ists" "step op (ipc, ist) = Some (opc, ost)" ..
   obtain icstack icregs icflag icrs where ist_split: "ist = (icstack, icregs, icflag, icrs)" by (rule prod_cases4)
@@ -137,7 +137,7 @@ proof -
     "(icstack, icregs, icflag, icrs) \<in> ?ists"
     "step op (ipc, (icstack, icregs, icflag, icrs)) = Some (opc, (ocstack, ocregs, ocflag, ocrs))" by auto
 
-  (* more properties can be added here if \<gamma>_stackless gets updated *)
+  (* more properties can be added here if \<gamma>_smart gets updated *)
   from ist_step(1) ist_split have ist_props: "icregs \<in> \<gamma>_regs iaregs" "icflag \<in> \<gamma>_power_bool iaflag" by auto
 
   show ?thesis 
@@ -152,13 +152,13 @@ proof -
       case BTrue
       from this have "icflag = True" using ist_props by simp
       from this JMPZ ist_split_step(2) have "opc = Suc ipc" using step_jmpz_true(4) by blast
-      from this BTrue JMPZ have "lookup (step_stackless op ipc (Some (Stackless iaregs iaflag))) opc = Some (Stackless iaregs iaflag)" using single_lookup by simp
+      from this BTrue JMPZ have "lookup (step_smart op ipc (Some (Smart iaregs iaflag))) opc = Some (Smart iaregs iaflag)" using single_lookup by simp
       then show ?thesis using ist_split flag_preserve ist_step(1) ost_split regs_preserve by simp
     next
       case BFalse
       from this have "icflag = False" using ist_props by simp
       from this JMPZ ist_split_step(2) have "opc = target" using step_jmpz_false(4) by blast
-      from this BFalse JMPZ have "lookup (step_stackless op ipc (Some (Stackless iaregs iaflag))) opc = Some (Stackless iaregs iaflag)" using single_lookup by simp
+      from this BFalse JMPZ have "lookup (step_smart op ipc (Some (Smart iaregs iaflag))) opc = Some (Smart iaregs iaflag)" using single_lookup by simp
       then show ?thesis using ist_split flag_preserve ist_step(1) ost_split regs_preserve by simp
     next
       case BBoth
@@ -166,17 +166,17 @@ proof -
       proof (cases icflag)
         case True
         from this JMPZ ist_split_step(2) have "opc = Suc ipc" using step_jmpz_true(4) by (metis(full_types))
-        from this BBoth JMPZ have lookup: "Some (Stackless iaregs iaflag) \<le> lookup (step_stackless op ipc (Some (Stackless iaregs iaflag))) opc" using deep_merge_lookup
-          by (metis insert_iff step_stackless.simps(2) step_stackless_base.simps(3))
-        have "ost \<in> \<gamma>_stackless (Some (Stackless iaregs iaflag))" using ist_split flag_preserve ist_step(1) ost_split regs_preserve by simp
-        from this lookup show ?thesis using gamma_stackless_mono by blast
+        from this BBoth JMPZ have lookup: "Some (Smart iaregs iaflag) \<le> lookup (step_smart op ipc (Some (Smart iaregs iaflag))) opc" using deep_merge_lookup
+          by (metis insert_iff step_smart.simps(2) step_smart_base.simps(3))
+        have "ost \<in> \<gamma>_smart (Some (Smart iaregs iaflag))" using ist_split flag_preserve ist_step(1) ost_split regs_preserve by simp
+        from this lookup show ?thesis using gamma_smart_mono by blast
       next
         case False
         from this JMPZ ist_split_step(2) have "opc = target" using step_jmpz_false(4) by (metis(full_types))
-        from this BBoth JMPZ have lookup: "Some (Stackless iaregs iaflag) \<le> lookup (step_stackless op ipc (Some (Stackless iaregs iaflag))) opc" using deep_merge_lookup
-          by (metis insert_iff step_stackless.simps(2) step_stackless_base.simps(3))
-        have "ost \<in> \<gamma>_stackless (Some (Stackless iaregs iaflag))" using ist_split flag_preserve ist_step(1) ost_split regs_preserve by simp
-        from this lookup show ?thesis using gamma_stackless_mono by blast
+        from this BBoth JMPZ have lookup: "Some (Smart iaregs iaflag) \<le> lookup (step_smart op ipc (Some (Smart iaregs iaflag))) opc" using deep_merge_lookup
+          by (metis insert_iff step_smart.simps(2) step_smart_base.simps(3))
+        have "ost \<in> \<gamma>_smart (Some (Smart iaregs iaflag))" using ist_split flag_preserve ist_step(1) ost_split regs_preserve by simp
+        from this lookup show ?thesis using gamma_smart_mono by blast
       qed
     qed
   next
@@ -249,25 +249,25 @@ qed
 end
 
 sublocale AbsStack \<subseteq> AbsInt
-  where \<gamma> = "\<gamma>_stackless"
-    and ai_step = step_stackless
+  where \<gamma> = "\<gamma>_smart"
+    and ai_step = step_smart
 proof (standard, goal_cases)
   case (1 a b)
-  then show ?case by (rule gamma_stackless_mono)
+  then show ?case by (rule gamma_smart_mono)
 next
-  case 2 show ?case by (rule gamma_stackless_top)
+  case 2 show ?case by (rule gamma_smart_top)
 next
   case (3 op ipc a pc)
-  then show ?case using step_stackless_nonbot_correct
+  then show ?case using step_smart_nonbot_correct
   proof (cases "a = \<bottom>")
     case True
     then show ?thesis by simp
   next
     case False
-    have "lookup (collect_step op ipc (\<gamma>_stackless (Some (Stackless regs flag)))) pc
-          \<le> \<gamma>_stackless (lookup (step_stackless op ipc (Some (Stackless regs flag))) pc)" for regs flag
-      using step_stackless_nonbot_correct by blast
-    from this False show ?thesis by (metis \<gamma>_stackless.elims bot_option_def)
+    have "lookup (collect_step op ipc (\<gamma>_smart (Some (Smart regs flag)))) pc
+          \<le> \<gamma>_smart (lookup (step_smart op ipc (Some (Smart regs flag))) pc)" for regs flag
+      using step_smart_nonbot_correct by blast
+    from this False show ?thesis by (metis \<gamma>_smart.elims bot_option_def)
   qed
 next
   case (4 op ipc pc)
